Use a real crash effect for async disks
All proofs are now fixed, using predicate transformers to state
recovery/crash post conditions with arbitrary precondition predicates.

src/Disk/AsyncDisk.v
@@ -46,6 +46,7 @@ Qed.
 Record covered (d:disk) (d':disk) : Prop :=
   is_covered
     { covered_size_eq: size d = size d';
+      (* TODO: express this as a match, automation will be way simpler *)
       covers_pointwise: forall a bs bs',
           d a = Some bs ->
           d' a = Some bs' ->
@@ -120,6 +121,72 @@ Theorem oldest_size_eq : forall d,
     size (oldest d) = size d.
 Proof.
   auto.
+Qed.
+
+Definition then_oldest (P: disk -> Prop) : disk -> Prop :=
+  fun d' => exists d, P d /\ covered (oldest d) d'.
+
+Lemma then_oldest_oldest : forall (F: disk -> Prop) d,
+    F d ->
+    then_oldest F (oldest d).
+Proof.
+  unfold then_oldest; intros.
+  exists d; intuition.
+Qed.
+
+Lemma covers_nil_tl : forall b0 b0' bs',
+    covers (necons b0 nil) (necons b0' bs') ->
+    b0 = b0' /\
+    (forall b, List.In b bs' -> b = b0).
+Proof.
+  intros.
+  inversion H; subst; simpl in *; intuition.
+  destruct (H1 b); auto; try contradiction.
+Qed.
+
+Lemma last_in_list : forall A (l: list A) (a:A),
+    List.In (List.last l a) l \/ List.last l a = a.
+Proof.
+  induction l; simpl; intros; eauto.
+  destruct (IHl a0); subst.
+  destruct l; eauto.
+  destruct l; eauto.
+Qed.
+
+Lemma covers_first_last : forall bs bs' bs'',
+    covers (keepFirst bs) bs' ->
+    covers (keepLast bs') bs'' ->
+    covers (keepFirst bs) bs''.
+Proof.
+  destruct bs, bs', bs'';
+    unfold keepFirst, keepLast;
+    simpl;
+    intros.
+  apply covers_nil_tl in H; intuition subst.
+  assert (List.last xs0 x0 = x0).
+  destruct (last_in_list xs0 x0); eauto.
+  congruence.
+Qed.
+
+Theorem covered_flush_oldest : forall d d' d'',
+    covered (flush d) d' ->
+    covered (oldest d') d'' ->
+    covered (flush d) d''.
+Proof.
+  intros.
+  destruct H, H0.
+  econstructor; intros.
+  - pose proof (oldest_size_eq d').
+    congruence.
+  - simpl in *.
+    specialize (covers_pointwise0 a).
+    specialize (covers_pointwise1 a).
+    destruct matches in *;
+      try solve [ exfalso; eauto using same_size_disks_not_different ].
+    inversion H; subst.
+    specialize (covers_pointwise0 _ _ ltac:(eauto) ltac:(eauto)).
+    specialize (covers_pointwise1 _ _ ltac:(eauto) ltac:(eauto)).
+    eauto using covers_first_last.
 Qed.
 
 (* partial flush at each address; expressed for convenient inversion *)
